# 反演问题

## **单位根反演**


$$
[n|k] = \frac{1}{n}\sum_{i = 0}^{n - 1}\omega_n^{ik}
$$
 证明：

若 $[n|k] = 0$，则
$$
\begin{aligned}
\sum_{i = 0}^{n - 1}\omega_n^{ik} 
=\dfrac{1 - \omega_n^{nk}}{1 - \omega_n^{k}} = 0\newline
\end{aligned}
$$
否则有
$$
\omega_n^{ik} = 1
$$
因此原式为1 。

### 例题

#### [2021HDU多校第五场B](https://acm.hdu.edu.cn/showproblem.php?pid=7013)

#### 题意

简化后的题意即对于所有的 $0 \le i, j < n$ 求
$$
\sum_{p = 0}^{L}\sum_{q = 0}^{L - p}[n|p - i][n|q - j]C_{L}^{p}C_{L - p}^{q}(k - 2)^{L - p - q}
$$
$L \le 10^{18}, n \le 500, k \le 26$

#### 题解

考虑转化


$$
\begin{aligned}
ans_{ij} &=\sum_{p = 0}^{L}\sum_{q = 0}^{L - p}[n|p - i][n|q - j]C_{L}^{p}C_{L - p}^{q}(k - 2)^{L - p - q} \newline
 &=\sum_{p = 0}^{L}\sum_{q = 0}^{L - p} \frac{1}{n}\sum_{I = 0}^{n - 1}\omega_{n}^{I(p - i)} \frac{1}{n}\sum_{J = 0}^{n - 1}\omega_{n}^{J(q - j)}C_L^p C_{L - p}^q(k - 2)^{(L - p - q)}\newline
 &=\frac{1}{n^2}\sum_{p = 0}^{L}\sum_{q = 0}^{L - p}\sum_{I = 0}^{n - 1}\sum_{J = 0}^{n - 1}\omega_n^{Ip}\omega_n^{Jq}C_L^pC_{L - p}^q(k - 2)^{L - p - q}\omega_n^{-Ii}\omega_n^{-Jj}\newline
 &=\frac{1}{n^2}\sum_{I = 0}^{n - 1}\sum_{J = 0}^{n - 1}(\omega_n^{I} + \omega_n^{J} + k - 2)^L\omega_n^{-Ii}\omega_n^{-Jj}
\end{aligned}
$$


令 $A_{iI} = \omega_n^{-Ii}, B_{IJ} = \frac{1}{n^2}(\omega_n^{I} + \omega_n^{J} + k - 2)^L, C_{Jj} = \omega_n^{-Jj}$

可知 $ans = A\times B \times C$

注：$\omega_n^{1} = g^{\frac{P - 1}{n}}$